src/cddl/pulse/CDDL.Pulse.AST.Parse.fst
@@ -1,6 +1,7 @@
 module CDDL.Pulse.AST.Parse
 include CDDL.Pulse.AST.Base
 include CDDL.Pulse.AST.Parse.ElemType
+include CDDL.Pulse.Parse.ArrayGroup
 include CDDL.Pulse.AST.Types
 open Pulse.Lib.Pervasives
 module Cbor = CBOR.Spec.API.Format
@@ -54,14 +55,66 @@ let ancillary_parse_env_extend
   end
   else None
 
+[@@sem_attr]
+let ancillary_parse_array_group_env
+  (#cbor_t: Type)
+  (vmatch: perm -> cbor_t -> Cbor.cbor -> slprop)
+  (#cbor_array_iterator_t: Type0)
+  (cbor_array_iterator_match: perm -> cbor_array_iterator_t -> list Cbor.cbor -> slprop)  
+  (#se: sem_env)
+  (#s_env: target_type_env se.se_bound)
+  (r_env: rel_env s_env)
+  (sp_env: spec_env se s_env.te_type)
+= (t: group) -> (t_wf: ast0_wf_array_group t { spec_wf_array_group se t t_wf }) -> option (impl_array_group cbor_array_iterator_match (array_group_sem se t) & impl_zero_copy_array_group cbor_array_iterator_match (spec_of_wf_array_group sp_env t_wf).ag_parser (impl_type_sem vmatch cbor_array_iterator_match r_env (target_type_of_wf_array_group t_wf)).sem_rel)
+
+[@@sem_attr]
+let ancillary_parse_array_group_env_extend
+  (#cbor_t: Type)
+  (#vmatch: perm -> cbor_t -> Cbor.cbor -> slprop)
+  (#cbor_array_iterator_t: Type0)
+  (#cbor_array_iterator_match: perm -> cbor_array_iterator_t -> list Cbor.cbor -> slprop)  
+  (#se: sem_env)
+  (#s_env: target_type_env se.se_bound)
+  (#r_env: rel_env s_env)
+  (#sp_env: spec_env se s_env.te_type)
+  (env1: ancillary_parse_array_group_env vmatch cbor_array_iterator_match r_env sp_env)
+  (#se2: sem_env)
+  (#s_env2: target_type_env se2.se_bound)
+  (r_env2: rel_env s_env2 {
+    rel_env_included r_env r_env2
+  })
+  (sp_env2: spec_env se2 s_env2.te_type {
+    spec_env_included sp_env sp_env2
+  })
+: Tot (ancillary_parse_array_group_env vmatch cbor_array_iterator_match r_env2 sp_env2)
+= fun t t_wf ->
+  if bounded_wf_array_group se.se_bound t t_wf
+  then begin
+    (env1 t t_wf)
+  end
+  else None
+
 module U64 = FStar.UInt64
 module U8 = FStar.UInt8
 module I64 = FStar.Int64
 module V = CDDL.Pulse.AST.Validate
 module SZ = FStar.SizeT
 
+noeq
+type ask_for =
+| AskForType: t: typ -> ast0_wf_typ t -> ask_for
+| AskForArrayGroup: t: group -> ast0_wf_array_group t -> ask_for
+
+let ask_for_spec
+  (se: sem_env)
+  (a: ask_for)
+: Tot prop
+= match a with
+  | AskForType t t_wf -> spec_wf_typ se true t t_wf
+  | AskForArrayGroup t t_wf -> spec_wf_array_group se t t_wf
+
 [@@sem_attr]
-let rec impl_zero_copy_type
+let rec impl_zero_copy_wf_type
   (#cbor_t #t2 #t_arr #t_map: Type0)
   (#vmatch: (perm -> cbor_t -> Cbor.cbor -> slprop))
   (#vmatch2: (perm -> t2 -> (Cbor.cbor & Cbor.cbor) -> slprop))
@@ -75,22 +128,23 @@ let rec impl_zero_copy_type
   (sp_env: spec_env se s_env.te_type)
   (p_env: parse_env vmatch r_env sp_env)
   (ancillary: ancillary_parse_env vmatch cbor_array_iterator_match r_env sp_env)
+  (ancillary_ag: ancillary_parse_array_group_env vmatch cbor_array_iterator_match r_env sp_env)
   (#t: typ)
   (t_wf: ast0_wf_typ t {
     spec_wf_typ se true t t_wf /\ SZ.fits_u64
   })
-: Pure (either (impl_zero_copy_parse vmatch (spec_of_wf_typ sp_env t_wf).parser (impl_type_sem vmatch cbor_array_iterator_match r_env (target_type_of_wf_typ t_wf)).sem_rel) (t': typ & ast0_wf_typ t'))
+: Pure (either (impl_zero_copy_parse vmatch (spec_of_wf_typ sp_env t_wf).parser (impl_type_sem vmatch cbor_array_iterator_match r_env (target_type_of_wf_typ t_wf)).sem_rel) (ask_for))
     (requires True)
     (ensures (fun res -> match res with
     | Inl _ -> True
-    | Inr (| t', t_wf' |) -> spec_wf_typ se true t' t_wf'
+    | Inr a -> ask_for_spec se a
     ))
     (decreases t_wf)
 = match t_wf with
   | WfTRewrite _ _ s ->
-    impl_zero_copy_type impl v_env r_env sp_env p_env ancillary s
+    impl_zero_copy_wf_type impl v_env r_env sp_env p_env ancillary ancillary_ag s
   | WfTTagged tg _ s ->
-    begin match impl_zero_copy_type impl v_env r_env sp_env p_env ancillary s with
+    begin match impl_zero_copy_wf_type impl v_env r_env sp_env p_env ancillary ancillary_ag s with
     | Inr ask -> Inr ask
     | Inl p ->
       begin match tg with
@@ -99,17 +153,17 @@ let rec impl_zero_copy_type
       end
     end
   | WfTChoice _ _ s1 s2 ->
-    begin match impl_zero_copy_type impl v_env r_env sp_env p_env ancillary s1 with
+    begin match impl_zero_copy_wf_type impl v_env r_env sp_env p_env ancillary ancillary_ag s1 with
     | Inr ask -> Inr ask
     | Inl p1 ->
-      begin match impl_zero_copy_type impl v_env r_env sp_env p_env ancillary s2 with
+      begin match impl_zero_copy_wf_type impl v_env r_env sp_env p_env ancillary ancillary_ag s2 with
       | Inr ask -> Inr ask
       | Inl p2 -> Inl (impl_zero_copy_choice (V.validate_typ impl v_env true _ s1) p1 p2)
       end
     end
   | WfTElem e -> Inl (impl_zero_copy_elem_type vmatch impl.cbor_get_major_type impl.cbor_destr_int64 impl.cbor_get_string impl.cbor_destr_simple e)
   | WfTDetCbor _ _ s ->
-    begin match impl_zero_copy_type impl v_env r_env sp_env p_env ancillary s with
+    begin match impl_zero_copy_wf_type impl v_env r_env sp_env p_env ancillary ancillary_ag s with
     | Inr ask -> Inr ask
     | Inl p ->
       Inl (impl_zero_copy_det_cbor impl.cbor_get_string impl.cbor_det_parse _ p)
@@ -125,3 +179,76 @@ let rec impl_zero_copy_type
   | WfTDef n -> Inl (p_env n)
   | WfTArray _ _ -> admit ()
   | WfTMap _ _ _ -> admit ()
+
+[@@sem_attr]
+let rec impl_zero_copy_wf_array_group
+  (#cbor_t #t2 #t_arr #t_map: Type0)
+  (#vmatch: (perm -> cbor_t -> Cbor.cbor -> slprop))
+  (#vmatch2: (perm -> t2 -> (Cbor.cbor & Cbor.cbor) -> slprop))
+  (#cbor_array_iterator_match: (perm -> t_arr -> list Cbor.cbor -> slprop))
+  (#cbor_map_iterator_match: (perm -> t_map -> list (Cbor.cbor & Cbor.cbor) -> slprop))
+  (impl: cbor_impl vmatch vmatch2 cbor_array_iterator_match cbor_map_iterator_match)
+  (#se: sem_env)
+  (v_env: V.validator_env vmatch se)
+  (#s_env: target_type_env se.se_bound)
+  (r_env: rel_env s_env)
+  (sp_env: spec_env se s_env.te_type)
+  (p_env: parse_env vmatch r_env sp_env)
+  (ancillary: ancillary_parse_env vmatch cbor_array_iterator_match r_env sp_env)
+  (ancillary_ag: ancillary_parse_array_group_env vmatch cbor_array_iterator_match r_env sp_env)
+  (#t: group)
+  (t_wf: ast0_wf_array_group t {
+    spec_wf_array_group se t t_wf /\ SZ.fits_u64
+  })
+: Pure (either (impl_zero_copy_array_group cbor_array_iterator_match (spec_of_wf_array_group sp_env t_wf).ag_parser (impl_type_sem vmatch cbor_array_iterator_match r_env (target_type_of_wf_array_group t_wf)).sem_rel) (ask_for))
+    (requires True)
+    (ensures (fun res -> match res with
+    | Inl _ -> True
+    | Inr a -> ask_for_spec se a
+    ))
+    (decreases t_wf)
+= match t_wf with
+  | WfAElem _ _ _ t_wf' ->
+    begin match impl_zero_copy_wf_type impl v_env r_env sp_env p_env ancillary ancillary_ag t_wf' with
+    | Inl pt ->
+      Inl (impl_zero_copy_array_group_item impl.cbor_array_iterator_next pt)
+    | Inr ask -> Inr ask
+    end
+  | WfAZeroOrOne _ t_wf' ->
+    begin match impl_zero_copy_wf_array_group impl v_env r_env sp_env p_env ancillary ancillary_ag t_wf' with
+    | Inr ask -> Inr ask
+    | Inl pe ->
+      Inl (impl_zero_copy_array_group_zero_or_one pe (V.validate_array_group impl v_env _ t_wf'))
+    end
+  | WfAZeroOrOneOrMore _ t_wf' g' ->
+    // HERE I need function pointers, so I MUST NOT do a recursive call
+    begin match ancillary_ag _ t_wf' with
+    | None -> Inr (AskForArrayGroup _ t_wf')
+    | Some (ve, pe) ->
+      begin match g' with
+      | GZeroOrMore _ ->
+        Inl (impl_zero_copy_array_group_zero_or_more impl.cbor_array_iterator_share impl.cbor_array_iterator_gather ve pe ())
+      | _ ->
+        Inl (impl_zero_copy_array_group_one_or_more impl.cbor_array_iterator_share impl.cbor_array_iterator_gather ve pe ())
+      end
+    end
+  | WfAConcat _ _ t_wf1 t_wf2 ->
+    begin match impl_zero_copy_wf_array_group impl v_env r_env sp_env p_env ancillary ancillary_ag t_wf1 with
+    | Inr ask -> Inr ask
+    | Inl pg1 ->
+      begin match impl_zero_copy_wf_array_group impl v_env r_env sp_env p_env ancillary ancillary_ag t_wf2 with
+      | Inr ask -> Inr ask
+      | Inl pg2 -> Inl (impl_zero_copy_array_group_concat impl.cbor_array_iterator_length impl.cbor_array_iterator_share impl.cbor_array_iterator_gather impl.cbor_array_iterator_truncate pg1 (V.validate_array_group impl v_env _ t_wf1) pg2 ())
+      end
+    end
+  | WfAChoice _ _ t_wf1 t_wf2 ->
+    begin match impl_zero_copy_wf_array_group impl v_env r_env sp_env p_env ancillary ancillary_ag t_wf1 with
+    | Inr ask -> Inr ask
+    | Inl pg1 ->
+      begin match impl_zero_copy_wf_array_group impl v_env r_env sp_env p_env ancillary ancillary_ag t_wf2 with
+      | Inr ask -> Inr ask
+      | Inl pg2 -> Inl (impl_zero_copy_array_group_choice pg1 (V.validate_array_group impl v_env _ t_wf1) pg2)
+      end
+    end
+  | WfARewrite _ _ t_wf2 ->
+    impl_zero_copy_wf_array_group impl v_env r_env sp_env p_env ancillary ancillary_ag t_wf2
