src/cddl/pulse/CDDL.Pulse.AST.Types.fst
@@ -97,20 +97,20 @@ let rec impl_type_sem
     let it = impl_type_sem vmatch cbor_array_iterator_match env t in {
       sem_impl_type =
         either
-          (slice it.sem_impl_type)
+          (vec_or_slice it.sem_impl_type)
           (array_iterator_t cbor_array_iterator_match it.sem_impl_type (Iterator.mk_spec it.sem_rel)) // HERE the relation on the element types is used in the implementation array type
           ;
       sem_rel =
         rel_either_left
-          (rel_slice_of_list it.sem_rel false)
+          (rel_vec_or_slice_of_list it.sem_rel false)
           (rel_array_iterator cbor_array_iterator_match (Iterator.mk_spec it.sem_rel))
           ;
     }
   | TTTable t1 t2 ->
     let it1 = impl_type_sem vmatch cbor_array_iterator_match env t1 in
     let it2 = impl_type_sem vmatch cbor_array_iterator_match env t2 in {
-      sem_impl_type = slice (it1.sem_impl_type & it2.sem_impl_type); // HERE we will plug support for iterable CBOR maps whose elements will be parsed wrt. it1.sem_rel, it2.sem_rel
-      sem_rel = rel_slice_of_table (target_type_eq s_env t1) it1.sem_rel it2.sem_rel
+      sem_impl_type = vec_or_slice (it1.sem_impl_type & it2.sem_impl_type); // HERE we will plug support for iterable CBOR maps whose elements will be parsed wrt. it1.sem_rel, it2.sem_rel
+      sem_rel = rel_vec_or_slice_of_table (target_type_eq s_env t1) it1.sem_rel it2.sem_rel false
     }
 
 let rel_env_included
